refactoring in process

poSTVM/poSTVM_parser_alt.thy
@@ -346,15 +346,44 @@ datatype stacked_func_block_var =
   InOutVar stacked_vars |
   InVar stacked_vars |
   OutVar stacked_vars
-datatype func_var =
-  Var stacked_vars |
-  InOutVar stacked_vars |
-  InVar stacked_vars |
-  OutVar stacked_vars
 
-type_synonym stacked_function_block = "func_block_name * stacked_func_block_var list * stacked_process list"
+datatype stacked_func_var = 
+  Var stacked_var_init
+| InOutVar stacked_var_init
+| InVar stacked_var_init
+| OutVar stacked_var_init
 
-type_synonym stacked_function = "func_name * basic_post_type * func_var list * stmt"
+type_synonym stacked_func_vars = "(id,stacked_func_var) fmap"
+
+text "Converting program vars to stacked version"
+definition stack_func_var :: "func_var \<Rightarrow> stacked_func_vars" where
+"stack_func_var var = 
+  (case var of
+    (func_var.Var (is_const, vars)) \<Rightarrow> (fmmap_keys (\<lambda>name val. stacked_func_var.Var (stack_var_init_decl val)) vars)
+  | (func_var.InOutVar vars) \<Rightarrow> (fmmap_keys (\<lambda>name val. stacked_func_var.InOutVar (stack_var_init_decl val)) vars) 
+  | (func_var.InVar vars) \<Rightarrow> (fmmap_keys (\<lambda>name val. stacked_func_var.InVar (stack_var_init_decl val)) vars)
+  | (func_var.OutVar vars) \<Rightarrow> (fmmap_keys (\<lambda>name val. stacked_func_var.OutVar (stack_var_init_decl val)) vars))"
+declare stack_func_var_def [simp]
+
+text "Converting program vars list to stacked version"
+definition stack_func_vars :: "func_var list \<Rightarrow> stacked_func_vars" where
+"stack_func_vars pl = (fold (\<lambda>val fm. (fmadd fm (stack_func_var val))) pl fmempty)"
+declare stack_func_vars_def [simp]
+
+
+type_synonym stacked_func_block = "func_block_name * stacked_func_block_var list * stacked_process list"
+
+type_synonym stacked_func = "func_name * basic_post_type * stacked_func_vars * stmt"
+
+definition stack_function :: "function_decl \<Rightarrow> stacked_func" where
+"stack_function fd = 
+  (let (f_name,val,vars,st_list) = fd
+  in (f_name,val,(stack_func_vars vars),(st_list_to_stmt st_list)))"
+declare stack_function_def [simp]
+
+definition stack_functions :: "function_decl list \<Rightarrow> (func_name,stacked_func) fmap" where
+"stack_functions fd_list = fmap_of_list (map (\<lambda>fd. (fst fd, stack_function fd)) fd_list)"
+declare stack_functions_def [simp]
 
 datatype stacked_global_var =
   Var stacked_var_init
@@ -375,7 +404,7 @@ definition stack_global_vars :: "global_var_decl list \<Rightarrow> stacked_glob
 declare stack_global_vars_def [simp]
 
 (*TO DO stacking configuration, function blocks and functions*)
-type_synonym stacked_model = "(configuration_decl option) * stacked_global_vars * (stacked_program list) * (function_block_decl list) * (function_decl list)"
+type_synonym stacked_model = "(configuration_decl option) * stacked_global_vars * (stacked_program list) * (function_block_decl list) * ((func_name,stacked_func)fmap)"
 
 text "Converting model declaration to stacked version"
 definition stack_model :: "model \<Rightarrow> stacked_model" where
@@ -387,7 +416,7 @@ definition stack_model :: "model \<Rightarrow> stacked_model" where
     (\<lambda>prog. (stack_program prog))
     prog_list),
   fb_list,
-  f_list))"
+  stack_functions f_list))"
 declare stack_model_def [simp]
 
 end
